\documentclass[12pt]{article}
\usepackage{my_preamble}

% Document Starts
\begin{document}

\maketitle 

\begin{abstract}
  Real Analysis the study of approximation on the reals.
\end{abstract}

\tableofcontents

\pagebreak
% <++>

\section{Cardinality}
\subsection{Brief Motivation}
We want to build a metric space to measure the distance between objects.

We need
\begin{enumerate}
  \item set $X$ of objects.
  \item need to measure closeness. func \(d:X\times X\to[0,\infty)\) s/t
    \begin{enumerate}
      \item \(d(x,y)=0\iff x=y\)
      \item \(d(x,y)=d(y,x)\)
      \item \(d(x,z)\le d(x,y)+d(y,z)\)
    \end{enumerate}
\end{enumerate}

We call \(d\) a metric on \(X\). \((X,d)\) is a \TB{metric space}.
\bboxex
\((\R,+'\circ^\circ(\sqrt{\,}^=)-)\) is a metric space. Note the BQN notation.
\ebox

\subsection{Function Theory}
\bbox
\begin{defn}[Injection] \label{defn:inj}
  Let \(A,B\) be non-empty sets. We say \(f:A\to B\) is injective \TB{iff}
  \(\forall a,b\in A\quad f(a)=f(b)\implies a=b\)
\end{defn}
\ebox

\bbox
\begin{defn}[Surjection] \label{defn:surj}
  \(f:A\to B\) is a surjection if \(\forall b\in B\quad\exists a\in A\st f(a)
  = b\).
\end{defn}
\ebox

\bbox
\begin{defn}[Bijective] \label{defn:bij}
  \(f:A\to B\) is bijective \TB{iff} its injective and surjective.
\end{defn}
\ebox


\bbox
\begin{defn}[Invertable]
  \(f:A\to B\) is invertable \TB{iff} \(\exists g:B\to A\st g(f(a))=a\T{ and }
  f(g(b))=b\quad\forall a\in A,\,b\in B\).
\end{defn}
\ebox
We write \(g=f^{-1}\) and call it "the" inverse.


\bbox
\begin{prop}
  \(f:A\to B\) is invertable \TB{iff} f is bijective.
\end{prop}
\ebox

\begin{proof}
  \((\implies)\) \(f\) is invertable. Suppose \(f(a)=f(b)\). We'll show \(a=b\).
  \[f^{-1}f(a))=f^{-1}f(b))\]
  \[\implies a=b\]
  
  Now we'll show \(\forall b\in B\;\exists a\in A\;f(a)=b\).
  \[a=f^{-1}(b)\implies\T{there is way to get from b to a, and it's }f^{-1}\]

  \((\limplies)\) Assume \(f\is(\T{bijective})\). We'll construct \(f\)'s
  inverse. For \(b\in B\) let \(a_b\) be the unique element of \(A\st f(a_b)=b\).
  \(a_b\) exists b/c of surjectivity of f, and it's unique b/c of injectivity.
  \[g:=\{g:A\to B,\,g(b)=a_b\}\]
  \[f(g(b))=f(a_b)=b\]
  \[g(f(a_b))=g(b)=a_b\]
  \[\implies g=f^{-1}\]
\end{proof}

\bbox
\begin{prop}
  \(\exists(\T{injection})\,f:A\to B\iff\exists(\T{surjection})\,g:B\to A\)
\end{prop}
\ebox

\bboxproof
\begin{proof}
  \((\implies)\) Suppose \(f:A\to B\is(\T{injective})\). Let \(b\in B\).
  
  Case 1: \(b\in f(A)\). 

  Let \(g(b)\) be the unique element of \(A\st f(g(b))=b\), unique b/c 
  \(f\is\TM{injective}\)

  Case 2: \(b\not\in f(A)\).

  Fix any \(z\in A\). Let \(g(b)=z\).
  
  \begin{equation*}
    \implies g(b)=\begin{cases}f^{=}(b)&b\in f(A)\\ z&b\not\in f(A)\end{cases}
  \end{equation*}

  We claim \(g\) is a surjection. 
  So we have to show
  \(\forall a\in A,\,\exists b\in B\st g(b)=a\)
  Let \(a\in A\st f(a)\in B\).
  \[g(f(a))\implies f(g(f(a)))=f(a)\]
  \[\TM{injective}\implies g(f(a))=a\]
  \[\implies g\is\TM{surjective}\]

  \(\limplies\) Suppose \((g:B\to A)\is\TM{surjective}\).
  \(\forall a\in A\T{ choose }b_a\in B\st g(b_a)=a\).
  \(f:=\{f:A\to B\quad f(a)=b_a\}\). Suppose
  \[f(x)=f(y)\]
  \[\implies b_x=b_y\]
  \[\implies g(b_x)=g(b_y)\]
  \[\implies x=y\]
  \[\implies f\is\TM{injective}\]
\end{proof}
\ebox

% lecture 2


\bbox
\begin{defn}[Powerset]
  Let \(X\) be a set. Then \(\PP(X):=\{A:A\subseteq X\}\), called
  the "\TB{powerset} of \(X\)."
\end{defn}
\ebox

\bboxex
\[X=\{a,b\}\]
\[\PP(X)=\{\emptyset,\{a\},\{b\},\{a,b\}\}\]
\ebox


\bbox
\begin{axim}[Choice]\label{axim:choice}
  Given \(X\neq\emptyset\exists\T{a choice func }f:\PP(X)\backslash
  \{\emptyset\}\to X\st f(A)\in A\;\forall\empty\neq A\subseteq A\).
\end{axim}
\ebox

\subsection{Cardinality}
\bboxex
\[A=\{a,b\},\;B=\{c,d,e,f\}\]
\[\T{Intuitively }|A|<|B|\]
\[f\is\TM{inj}:A\to B,\;f(a):=c,\;f(b):=d\]
\[\implies f\is\TM{inj}(A)\subset B\]
\[\implies |A|\le |B|\]
\ebox

\bbox
\begin{defn}[Ordering of Cardinality on Sets]
  \(A,B\) sets.
  \begin{enumerate}
    \item \(|A|\le|B|\iff\exists f\is\TM{inj}:A\to B\)
    \item \(|A|=|B|\iff\exists f\is\TM{bij}:A\to B\)
  \end{enumerate}
\end{defn}
\ebox
\bboxex
\[|\N|\le|\Z|\limplies f\is\TM{inj}:\N\to\Z,\;f(n):=n\]
\begin{equation*}
  f\is\TM{bij}:\N\to\Z:f(n):=
  \begin{cases}
    2n+2&:n\ge0\\
    2(-n)-1&:n<0
  \end{cases}\implies|\N|=|\Z|
\end{equation*}
\[h\is\TM{bij}:\R\to(0,1):h(x):=\frac{\mathrm{arctan}(x)+\pi/2}\pi\implies|\R|=|(0,1)|\]
\ebox

\bbox
\begin{thm}[Cantor-Schroeder-Berstien (CSB)] \label{thm:CSB}
  if \(|A|\le|B|\) and \(|B|\le|A|\) then \(|A|=|B|\).
\end{thm}
\ebox


\bbox
\begin{lem}[Phi has a Fixed Point]\label{lem:phi_fixed_pt}
  \(X\) set. Suppose \(\exists\phi:\PP(X)\to\PP(X)\st\phi(A)\subseteq\phi(B)
  \T{ if }A\subseteq B\subseteq X\). Then
  \[\exists F\subseteq X\st\phi(F)=F\]
\end{lem}
\ebox

\bboxproof
Let \(F=\bigcup_{A\subseteq X:A\subseteq\phi(A)}A\).
\bboxnote
\TB{Note:} \(\emptyset\subseteq X\;\&\;\emptyset\subseteq\phi(\emptyset)\)
\ebox
\TB{Claim:} \(F=\phi(F)\).
Take \(A\subseteq X\) with \(A\subseteq\phi(A)\). Then \(A\subseteq F\).
\[\implies\phi(A)\subseteq\phi(F)\]
\[\implies A\subseteq\phi(F)\]
\[\implies\bigcup_{A\subseteq X:A\subseteq\phi(A)}A\subseteq\phi(F)\quad
\T{(by properties of unions)}\]
\[\implies F\subseteq\phi(F)\]
Further,
\[F\subseteq \phi(F)\implies\phi(F)\subseteq\phi(\phi(F))\]
\[\implies\phi(F)\in\{A\subseteq X:A\subseteq\phi(A)\}\]
For this step, let \(\phi(F)=B\) and notice that \(B\subseteq\phi(B)\). So
its in the set above.
\[\implies\phi(F)\subseteq\bigcup_{A\subseteq X:A\subseteq\phi(A)}A=F\]

\[\implies F=\phi(F)\]
\ebox

\bboxex
\TB{To motivate (CSB)~\cref{thm:CSB}:} prove that \(|N|=|N\times N|\).
\[f\is\TM{inj}:\N\to\N\times\N,\;f(n):=(n,1)\]
\[g\is\TM{inj}:\N\times\N\to\N,\;g((n,m)):=2^n3^m\]
By (CSB) \(|\N|=|\N\times\N|\).
\ebox

% lecture 3

\bboxproof
\begin{proof}[Proof of (CSB)~\cref{thm:CSB}]
  Let \(f,g\is\TM{inj}:A:B\). For \(X\subseteq Y\subseteq A\)
\[f(X)\subseteq f(Y)\]
\[\implies B\backslash f(Y)\subseteq B\backslash f(X)\]
\[\implies g(B\backslash f(Y))\subseteq g(B\backslash f(X))\]
\[\implies A\backslash g(B\backslash f(X))\subseteq A\backslash g(B\backslash f(Y))\]
This letting \(\phi:\PP(A)\to\PP(A):\phi(x):=A\backslash g(B\backslash f(x))\)
insures it preserves \(\subseteq\).
So by the \cref{lem:phi_fixed_pt}, \(\exists F\subseteq A
\st F=\phi(F)=A\backslash g(B\backslash f(F))\). In particular, \(A
\backslash F=g(B\backslash f(F))\implies g:B\backslash f(F)\to A\backslash F
:\is\TM{bij}\).
\bboxnote
\TB{Note.} It's a surjection b/c everyone in \(A\backslash F\) gets mapped to
b/c it's the image if \(g(B\backslash f(F))\).
\ebox
Moreover, \(\inv g:A\backslash F\to B\backslash f(F)\) is a bijection, and
\(f:F\to f(F)\) is a bijection (for the same reason as above; restriction of
domain of an injective function is injective, and a function that maps to its image is
automatically a surjection). Hence
\begin{equation*}
  h:A\to B:h(x):=
  \begin{cases}
    \inv g(x) &:x\in A\backslash F\\
    f(x) &:x\in F
  \end{cases}
\end{equation*}
\end{proof}
\ebox

\bboxex
Show \(|\Q|=|\N|\).
\bboxproof
\begin{proof}
  \[f:\N\to\Q:f(x):=x\implies|\N|\le|\Q|\]
  \(q\in\Q\) can be written in the form \(q=\frac m n,\;m\in\Z,\,n\in\N\).
  \[g:\Q\to\Z\times\N:g(q):=(m,n)\;:\;q=\frac m n\]
  \[\implies|\Q|\le|\Z\times\N|=|\N\times\N|=|\N|\]
  So by (CSB) \cref{thm:CSB}, \(|\Q|=|\N|\).
\end{proof}
\ebox
\ebox


\bbox
\begin{defn}[Finite, Countably Infinite, Countable]
  \(\,\)\begin{enumerate}
    \item a set \(A\) is \TB{finite} \TU{iff} \(|A|=|\{1,2,\dots,n\}|\)
      for some \(n\in\N\). In this case, \(|A|=n\).
    \item \(|\emptyset|:=0\)
    \item \(A\) is \TB{countably infinite} \TU{iff} 
      \(|A|=|\N|:=\aleph_0\).
    \item \(A\) is countable \TU{iff} \(A\) is finite or ctbly infinite.
  \end{enumerate}
\end{defn}
\ebox

\bboxex
\[|\N|=|\Z|=|\N\times\N|=|\Q|=\aleph_0\]
\ebox


\bbox
\begin{prop}[Aleph Null is the Smallest Infinity]\label{prop:aleph_null_small}
  If \(A\) is infinite, then \(|\N|\le|A|\).
\end{prop}
\ebox

\bboxproof
\begin{proof}
  By (Choice) \cref{axim:choice}, \(\exists f:\PP(A)\backslash\{\emptyset\}\to
  A\st f(X)\in X,\;\forall\emptyset\neq X\subseteq A\).
  \begin{equation*}
    \begin{split}
      \T{Let }a_1&=f(A)\in A\\
      a_2&=f(A\backslash\{a_1\})\in A\backslash\{a_1\}\\
         &\vdots
    \end{split}
  \end{equation*}
  \(\implies\aleph_0=|\{a_1,\dots\}|\le|A|\).
\end{proof}
\ebox

\bbox
\begin{prop}[The Reals are Uncountable]\label{prop:uncountable_reals}
\(\R\) is uncountable. So \(\not\exists f\is\TM{bij}:\N\to\R\).
\bboxproof
  \begin{proof} \TB{Cantor's Diagonal Element Proof.} 
    Since \(|\R|=|(0,1)|\), we'll show that \((0,1)\) is uncountable.

    For contradiction, assume that there exists a bijection \(f:\N\to(0,1)\).

    So let's say
    \begin{equation*}
      \begin{split}
        f(1)&=0.a_{11}a_{12}a_{13}\cdots\\
        f(2)&=0.a_{21}a_{22}a_{23}\cdots\\
        f(3)&=0.a_{31}a_{32}a_{33}\cdots\\
        \vdots&=\vdots
      \end{split}
    \end{equation*}
    Where we avoid repeated nines.

    Choose \(b_i\in\{1,\dots,8\}\st b_i\neq a_{ii}\).
    \[\implies\not\exists n\in\N,\;f(n)=0.b_1b_2b_3\cdots\]
    Thats a contradiction.
  \end{proof}
\ebox
\end{prop}
\ebox


\bbox
\begin{defn}[Continuum]\label{defn:continuum}
  We write \(|\R|=c\), where \(c\) stands for \TB{continuum}.
\end{defn}
\ebox

So we have 3 cardinals: \(n,\aleph_0,c\).


\bbox
\begin{axim}[Continuum Hypothesis]\label{axim:continuum_hypth}
  If \(A\) is a set with \(\aleph_0\le|A|\le c\), then
  \(\aleph_0=|A|\) or \(|A|=c\).
\end{axim}
\ebox

\subsection{Cardinality of Power Sets}


\bbox
\begin{prop}
  If \(|A|=n\), then \(|\PP(A)|=2^n\).
\end{prop}
\ebox
\bboxproof
\begin{proof}[Proof]
  \[|\PP(A)|=\sum_{k=1}^n\binom nk=(1+1)^n=2^n\]
\end{proof}
\ebox


% lecture 4



\bbox
\begin{defn}[Cartesian Product]\label{defn:cartesian_product}
  Let \(I\) be a set. \(\forall i \in I\;\T{Let }A_i\is\TM{set}\implies
  \prod_{i\in I}A_i:=\{f|f:I\to\bigcup A_i,\;f(i)\in A_i\}\)
\end{defn}
\ebox


\bboxnote
\[f(i)\in A_i\]
\[I=\N\implies f:\N\to\bigcup A_i:f(i):\!\in A_i\equiv(f(1),f(2),\dots)\]
\ebox

\bbox
\begin{defn}[Set Power]\label{defn:set_power}
  \(A,B\is\TM{set}\implies A^B=\{f:B\to A\}\)
  \[|A|^{|B|}:=\left|A^B\right|=|\{f:B\to A\}|\]
\end{defn}
\ebox

\bbox
\begin{prop}[Cardinality of a Power Set]\label{prop:card_of_powerset}
  if \(X\is\TM{set}\), \(\PP(X)=2^{|X|}=|\{f:X\to\{0,1\}\}|\).
\end{prop}
\ebox

\bboxproof
\begin{proof}
  \begin{equation*}
    \begin{split}
      \phi:\PP(X)\to\{f:X\to\{0,1\}\}:\phi(A)&:=\chi_A\\
      \chi_A:X\to\{0,1\}:\chi_A(x)&:=
      \begin{cases}
        1 &: x\in A\\
        0 &: x\not\in A
      \end{cases}
    \end{split}
  \end{equation*}
  Show \(\phi\is\TM{bij}\). First show it's injective.
  \[\phi(A)=\phi(B)\]
  \[\implies\chi_A=\chi_B\] % :'<,'>s/(\(.\))/_\1/g
  \[\implies A=B\implies\phi\is\TM{inj}\] % :'<,'>s/(\(.\))/_\1/g
  Now show it's surjective. \(\forall f\in\{f:X\to\{0,1\}\}\;\exists P\in \PP(X)\st
  \phi(P)=f\).
  \[\T{Let }\inv f(\{0,1\})=\inv F\]
  \[\implies \chi_{\inv F}:\inv F\to\{0,1\}\]
  \[\implies\chi_{\inv F}=\phi(\inv F)\T{ w/ }\phi(\inv F)=f\]
  \[\inv F\subseteq X\implies \inv F\in\PP(X)\implies \phi\is\TM{surj}\]
\end{proof}
\ebox


\bbox
\begin{prop}[The Powerset is Larger than the Set]\label{prop:powerset_big}
  If \(X\is\TM{set}\), then \(|X|<|\PP(X)|\).
\end{prop}
\ebox

\bboxproof
\begin{proof}
  Show \(|X|\le|\PP(X)|\). \(f(x)=\{x\}\is\TM{inj}\implies |X|\le|\PP(X)|\). 

  For the sake on contradiction, assume there is a surjection \(g:X\to\PP(X)\).
  Consider \(B:=\{x\in X:x\not\in g(x)\}\). Hence there must be (by surjectivity of \(g\))
  \(z\in X\st g(z)=B\). Someone has to map to it.
  \[z\in B\implies z\not\in g(z)=B\]
  \[z\not\in B\implies z\in g(z)=B\]
  This is a contradiction. So \(|X|<|\PP(X)|\).
\end{proof}
\ebox

\bboxnote\label{note:infinite_infinities}
\TB{Infinite Infinities}. \(|\N|<|\PP(\N)|<|\PP(\PP(\N))|<\dots\)
\ebox

\bbox
\begin{prop}[The Natural Powerset Cardinal is the Continuum Cardinal]\label{prop:abs_pp_n_is_abs_r}
  \(|\PP(\N)|=c\) \((\equiv 2^{\aleph_0}=c\equiv|\{0,1\}|^{|\N|}=|\R|)\)
\end{prop}
\ebox

\bboxproof
\begin{proof}\(\,\)
  \bboxnote
  We'll use the continuum hypthesis, however there's an alternative proof in 
  the course notes.
  \ebox
  Consider \(X=\{f:\N\to\{0,1\}\}\).
  \[\phi:X\to\R:\phi(f):=0.f(1)f(2)f(3)\dots\]
  We can see that \(\phi\) is injective. So
  \[2^{\aleph_0}=|X|\le|\R|=c\]
  Also, \(\aleph_0<2^{\aleph_0}\le c\). So by (CH), we know \(2^{\aleph_0}=c\).
\end{proof}
\ebox


\bboxproof
\begin{proof}[Proof (without (CH))]
  \(\dots\)
\end{proof}
\ebox

\subsection{Cardinal Arithmetic}

\bbox
\begin{defn}
  \(A,B\is\TM{sets}\)
  \begin{enumerate}
    \item \(A\cap B=\emptyset\implies|A|+|B|:=|A\cup B|\)
    \item \(|A|\cdot|B|:=|A\times B|\)
    \item \(|A|^{|B|}:=|\{f:B\to A\}|\)
  \end{enumerate}
\end{defn}
\ebox

\bboxex
\TB{Example.} \(\aleph_0+\aleph_0=\aleph_0\). Let \(A=\{a_1,\dots\}\),
\(B=\{b_1,\dots\}\), so that \(|A|=|B|=\aleph_0\), and \(A\cap B=\emptyset\).

Then \(\phi:A\cup B\to\N:
\phi(a_i):=2i,\;
\phi(b_i):=2i-1\).
This is a bijection.
Hence
\(|A\cup B|=\aleph_0\).
\ebox

\bboxex
\TB{Example.} \(\aleph_0+c=c\).

\(\aleph_0=|\N|,\;|(0,1)|=c\).
\[(0,1)\subseteq\N\cup(0,1)
\subseteq\R\]
\[\implies c\le\aleph_0+c\le c\]
\[\implies \aleph_0+c=c\]
\ebox


\bbox
\begin{prop}[Cardinal Exponent Laws]
  \(A,B,C\is\TM{sets}\).
  \begin{enumerate}
    \item \((|A|^{|B|})^{|C|}
      = |A|^{|B|\cdot|C|}\)
    \item \((|A|^{|B|})(|A|^{|C|})
      = |A|^{|B|+|C|}\)
  \end{enumerate}
\end{prop}
\ebox

\bboxex
\TB{Example.} Show that \(c\cdot c=c\).
\[c\cdot c=(2^{\aleph_0})(2^{\aleph_0})
=2^{\aleph_0+\aleph_0}=2^{\aleph_0}=c\]
\ebox

% lecture 5


\bboxproof
\begin{proof}[Proof of 2.]
  We must show
  \[|\{f|f:B\cup C\to A\}|
  =|\{f|f:B\cup A\}\times\{f|f:B\to A\}|\]
  \[\T{Let }X:=\{f|f:B\to A\}\]
  \[\T{Let }Y:=\{f|f:C\to A\}\]
  \[\T{Let }Z:=\{f|f:B\cup C\to A\}\]
  So, equivically we need to show \(|Z|=|X\times Y|\).
  
  Consider \(\varphi(f,g)(x)=\begin{cases}f(x)&x\in B\\ g(x)&y\in C\end{cases}\).
  \[\varphi(f_1,g_1)=\varphi(f_2,g_2)\]
  \[\implies\forall x\in B\cup C,\;
  \varphi(f_1,g_1)(x)=\varphi(f_2,g_2)(x)\]
  \[\implies\forall x\in B,\;f_1(x)=f_2(x)\implies f_1=f_2\]
  \[\implies\forall x\in C,\;g_1(x)=g_2(x)\implies g_1=g_2\]

  Consider \(h:B\cup C\to A\). Let \(f=h|_B,\;g=h|_C\). Then
  \(\varphi(f,g)=h\).

  So \(\varphi\) is bijective, so proposition 2 holds.
\end{proof}
\ebox


\bboxex
\TB{Example:} \(c^{\aleph_0}=(2^{\aleph_0})^{\aleph_0}
=2^{\aleph_0\cdot\aleph_0}=2^{\aleph_0}=c\).
\ebox

\section{Topology}
\subsection{Metric Spaces}

\bbox
\begin{defn}[Metric Space]\label{defn:metric_space}
  \(X\is\TM{set}\). A metric on \(X\) is a function
  \(d:X\times X\to[0,\infty)\st\)
  \begin{enumerate}
    \item \(d(x,y)=0\iff x=y\)
    \item \TB{Abelian:} \(d(x,y)=d(y,x)\)
    \item \TB{Triangle:} \(d(x,y)\le d(x,z)+d(z,y)\)
  \end{enumerate}
\end{defn}
\ebox


\bbox
\begin{defn}[Normed Vector Space (NVS)]\label{defn:nvs}
  Let \(V\is\TM{Vector\;Space}\) over \(\R\).
  A norm on \(V\) is a fn \(\|\cdot\|:V\to[0,\infty)\st\)
  \begin{enumerate}
    \item \(\|v\|=0\iff v=\vec 0\)
    \item \(\|\alpha v\|=|\alpha|\cdot\|v\|\)
    \item \(\|v+u\|\le\|v\|+\|u\|\)
  \end{enumerate}
\end{defn}
\ebox
\bboxex
\TB{BQN:} \(\|\times==|\circ l\cdot\|\circ r\quad\)\(|+\le\le+\Box|\)
\ebox


\bbox
\begin{prop}[NVS have trivial Metrics]\label{prop:nvs_have_trivial_metrics}
  Let \(V,\|\cdot\|\is\TM{NVS}\). \(d(v,w)=\|v-w\|\) is a metric on \(V\).
\end{prop}
\ebox

\subsection{Examples of Metric Spaces}


\bboxex
\begin{exam}[Discrete Metric]\label{exam:discrete_metric}
  \(X\is\TM{set}\).
  \[
    d(x,y)=\begin{cases}
    0&x=y\\ 1&x\neq y\end{cases}
  \]
\end{exam}
\ebox

\bboxex
\begin{exam}[Absolute Value Norm]\label{exam:absolute_value_norm}
  \((\R,|\cdot|)\is\TM{NVS}\)
\end{exam}
\ebox


\bboxex
\begin{exam}[Euclidean Norm]\label{exam:euclidean_norm}
  \((\R^n,\|\cdot\|_2)\is\TM{NVS}\) where \(\|x\|_2=\sqrt{\sum_{i=1}^n x_i^2}\).
\end{exam}
\ebox

\bboxex
\begin{exam}[P-Norm]\label{exam:p_norm}
  \(p\ge 1,\;(\R^n,\|\cdot\|_p)\is\TM{NVS}\) where
  \[\|x\|_p=\left(\sum_{i=1}^n|x_i|^p\right)^\frac1p\]
  \bboxnote
  \TB{Note:} see posted notes for the proof that this is a norm. OPTIONAL.
  \ebox
\end{exam}
\ebox

\bboxex
\begin{exam}[Infinity Norm]\label{exam:infinity_norm}
  \(p=\infty,\;(\R^n,\|\cdot\|_\infty)\is\TM{NVS}\) where
  \[\|x\|_\infty=\TR{max}\{|x_1|,\dots,|x_n|\}\]
\end{exam}
\ebox

\bboxex
\begin{exam}[P-Norm on Sequences of Reals]\label{exam:p_norm_on_sequences_of_reals}
  \(\R^\N:=\{f|f:\N\to\R\}=\{(a_n)_{n=1}^\infty:a_n\in\R\}\). For \(p\ge 1\),
  \begin{equation}
    \|x\|_p=\left(\sum_{n=1}^\infty|x_n|^p\right)^{\frac1p}
  \end{equation}

  \(l^p:=\{x\in\R:\|x\|_p<\infty\}\implies(l^p,\|\cdot\|_p)\is\TM{NVS}\). This
  is the p-norm on sequences of reals. Notice how this solve the divergence
  issue (by ignoring it lol).
\end{exam}
\ebox


\bboxex
\TB{Example:} \(l^1=\{x\in\R:\sum|x_i|<\infty\}\implies l^p\) is the set of
absolutly convergent sequences.
\ebox


\bboxex
\begin{exam}[Suprema Norm (Infinity Norm on Sequences of Reals)]\label{exam:suprema_norm}
  \(\|x\|_\infty=\sup\{|x_n|:n\in\N\}\).

  if we let \(l^\infty:=\{x\in\R^\N:\|x\|_\infty<\infty\}\), noting that
  \(l^\infty\) is the set of all bounded sequences, then 
  \((l^\infty,\|\cdot\|_\infty)\is\TM{NVS}\).
\end{exam}
\ebox

\bboxex
\begin{exam}[P-Norm on Function]\label{exam:p_norm_on_functions}
  \(C([a,b]):=\{f:[a,b]\to\R|f\is\TM{cts}\}\).
  \[\|f\|_p=\left(\int_a^b|f(x)|\md x\right)^{\frac1p},\;p\ge 1\]
\end{exam}
\ebox


\bboxex
\begin{exam}[Infinity Norm on Functions]\label{exam:infinity_norm_on_functions}
  \(\|f\|_\infty=\sup\{|f(x)|:x\in[a,b]\}\) 
\end{exam}
\ebox


\bboxex
\begin{exam}[Bounded Functions and the Infinity Norm are a NVS]\label{exam:bounded_functions_and_the_infinity_norm_are_a_nvs}
  \(\B([a,b])=\{f:[a,b]\to\R|f\is\TM{bd}\}\), \((\B([a,b]),\|\cdot\|_\infty)\is\TM{NVS}\).
\end{exam}
\ebox

% lecture 6

\bboxex
\begin{exam}[Sequence Metric]
  \(X=\R^\N=\{f|f:\N\to\R\}\). 
  \[d(x,y)=\sum_{i=1}^\infty\frac{|x_i-y_i|}{2^i(1+|x_i-y_i|)}\]
  \bboxproof
  \begin{proof}[Prove that d isn't induced by a metric.]
    If \(d(x,y)=\|x-y\|\) for some norm, then \(\|\alpha x-\alpha y\|
    =|\alpha|\|x-y\|\).
    \begin{align*}
      d(ax,ay)&=\sum_{i=1}^\infty\frac{|ax_i-ay_i|}{2^i(1+|ax_i-ay_i|)}\\
      d(ax,ay)&=\sum_{i=1}^\infty\frac{|a||x_i-y_i|}{2^i(1+|a||x_i-y_i|)}\\
      |a|d(x,y)&=|a|\sum_{i=1}^\infty\frac{|x_i-y_i|}{2^i(1+|x_i-y_i|)}\\
      |a|d(x,y)&=\sum_{i=1}^\infty\frac{|a||x_i-y_i|}{2^i(1+|x_i-y_i|)}\\
      \T{b/c }|a||x_i-y_i|&\neq |x_i-y_i|\\
                          &\implies\T{not induced by a norm}
    \end{align*}
  \end{proof}
  \ebox
\end{exam}
\ebox

\bboxex
\begin{exam}[Cantor Space]\label{exam:cantor_space}
  \(X=2^\N:=\{f|f:\N\to\{0,1\}\}\). 
  \[d(x,y)=\sum_{i=1}^\infty\frac{|x_i-y_i|}{2^i}\]
\end{exam}
\ebox

\bboxex
\begin{exam}[Hamming Distance]\label{exam:hamming_distace}
  \(X\is\TM{finite}\). \(A,B\in\PP(X)\). 
  \[d(A,B):=|A\triangle B|=|(A\cup B)\backslash(A\cap B)|\]
\end{exam}
\ebox

\bboxex
\begin{exam}[Hausdorff Metric]
  \(\HH=\{K\subseteq\R^n:K\T{ compact}\}\). Let 
  \(a\in A,\;b\in B,\;A,B\in\HH\).
  \[d(a,B)=\min\{\|a-b\|:b\in B\}\]
  \[d(b,A)=\min\{\|a-b\|:a\in A\}\]
  \[d(A,B)=\max\{\sup_{a\in A}d(a,B),\sup_{b\in B}d(b,A)\}\]

  \bboxnote
  \begin{note}
    \(\sup_{a\in A}d(a,B)\) represents the biggest shortest path between
    \(A\) and \(B\).
  \end{note}
  \ebox
\end{exam}
\ebox

\bboxnote
\begin{note}
  Metrics give a sense of convergence on a space.
\end{note}
\ebox

\bboxex
\begin{exam}[P-adic Metric]
  Let \(p\) be prime, \(X=\Q\).
  \[\T{Let }0\neq q\in X=\Q\quad q=p^a\frac nm\]
  \[\T{where }\gcd(n,m)=\gcd(p,n)=\gcd(p,m)=1\]
  \[|q|_p=\frac1{p^a},\;|0|_p=0\]
  \[d(q_1,q_2:=|q_1-q_2|_p\]
  \bboxnote
  \begin{note}
    This notion of distance implies the more factors of p, the closer.

    This gives a sense of optimizing for a certain adjective.

    These numbers aren't close using \(\|\cdot\|_2\), but are using
    the p-adic norm.
  \end{note}
  \ebox
\end{exam}
\ebox


\bbox
\begin{defn}[Subspace of a Metric Space]\label{defn:subspace_of_a_metric_space}
  \((X,d),\;Y\subseteq X\implies(Y,d)\). \((Y,d)\) is called a 
  \TB{subspace} of \((X,d)\).
\end{defn}
\ebox

\bbox
\begin{defn}
  \((X,d_1),\;(Y,d_2)\). Consider \((X\times Y,d)\) with
  \begin{align*}
    d((x_1,y_1),(x_2,y_2))&:=d_1(x_1,x_2)+d_2(y_1,y_2)\ (\T{1-norm})\\
    \T{or }d((x_1,y_1),(x_2,y_2))&:=\max\{d_1(x_1,x_2),d_2(y_1,y_2)\}\ (\infty\T{-norm})\\
  \end{align*}
\end{defn}
\ebox

\bboxex
\begin{exam}[Product Metric]\label{exam:product_metric}
  \((X_i,d_i)\;i\in\N\), \(X:=\prod_{n=1}^\infty X_i\). Let 
  \(x=(x_1,x_2,\dots)\T{ and }y=(y_1,y_2,\dots)\).
  \[d(x,y)=\sum_{i=1}^\infty\frac{d_i(x_i,y_i)}{2^i(1+d_i(x_i,y_i))}\]
\end{exam}
\ebox

\subsection{Convergence}

\bbox
\begin{defn}[Convergence of a Sequence]\label{defn:convergence_of_a_sequence}
  \((X,d),\;(x_n)\subseteq X\), and \(x\in X\).
  \bboxnote
  \begin{nota}
    \((x_n)\subseteq X\) means \((x_n)\) is a sequence in \(X\). 
  \end{nota}
  \ebox
  \[(x_n)\T{ conv to }x,\;x_n\to x\TB{ iff}\]
  \[\forall\e>0,\;\exists N\in\N\st\forall n\ge N,\;d(x_n,x)<\e\]
\end{defn}
\ebox


\bboxdefn
\begin{defn}[Divergence]\label{defn:divergence}
  \((x_n)\) diverges of \(\not\exists x\in X\st x_n\to x\).
\end{defn}
\ebox

\bboxnote
\begin{note}[Convergence is Distance going to Zero]
  \((X,d),\;(x_n)\in X,\;x\in x\). Then \(x_n\to x\) \TB{iff}
  \(d(x_n,x)\to 0\).
\end{note}
\ebox

\bboxdefn
\begin{defn}[Cauchy]
  \((X,d)\). \((x_n)\subseteq X\) is a cauchy seq \TB{iff}
  \[\forall\e>0,\;\exists N\in\N\st\forall n,m\ge N,\;
  d(x_n,x_m)<\e\]
\end{defn}
\ebox


\bboxprop
\begin{prop}[Convergence implies Cauchyness]
  \((X,d)\). If \((x_n)\subseteq X\) converges, then \((x_n)\) is cauchy.
\end{prop}
\ebox

\bboxproof
\begin{proof}[Epsilon/2]
  Suppose \((x_n)\to x\). Let \(\e>0\). So \(\exists N\st\forall n\ge N\), 
  \[d(x_n,x)<\gamma\]
  \begin{align*}
    d(x_n,x_m)&\le d(x_n,x)+d(x,x_m)\T{ by }\triangle\\
              &<\gamma+\gamma=2\gamma\\
              &:=2\frac\e2\\
              &=\e
  \end{align*}
\end{proof}
\ebox

\bboxexam
\begin{exam}[Cauchy doesn't imply Convergence]
  \(X=(0,1]\) with the std metric.
  \[\frac1n\to0\implies\left(\frac1n\right)\subseteq X\T{ is cauchy}\]
  \bboxnote
  \begin{note}
    I think this is trying to say that 1/n is cauchy in X, but 
    1/n \(\to\) 0, which is not in X, so it diverges (in X).
  \end{note}
  \ebox

\end{exam}
\ebox


% <++>
\end{document}


























% scrolloff buffer
